Lynx.lean
@@ -1,3 +1,5 @@
 import Lynx.Term
 import Lynx.Contract
 import Lynx.Modules.Erlang
+import Lynx.Modules.Enum
+import Lynx.Tactic
